tests/elab/vcgenDyLean.lean
@@ -336,12 +336,13 @@ theorem always_frame
   {α: Type}
   (f: Traceful α)
   (p: ProofTrace → Prop)
-  : PredTrans.Frames Lean.Order.meet (WP.wpTrans f) (Always' p) := by
-  intro Q E
-  simp only [PartialOrder.rel, my_meet_apply, and_imp, Subtype.forall]
-  dsimp only [wp, Always', WP.wpTrans]
-  simp [my_meet_apply]
-  grind [Trace.le_trans]
+  : PredTrans.Frames Lean.Order.meet (WP.wpTrans f) (Always' p)
+where
+  op_apply_le_apply_op Q E := by
+    simp only [PartialOrder.rel, my_meet_apply, and_imp, Subtype.forall]
+    dsimp only [wp, Always', WP.wpTrans]
+    simp [my_meet_apply]
+    grind [Trace.le_trans]
 
 grind_pattern always_frame => PredTrans.Frames Lean.Order.meet (WP.wpTrans f) (Always' p)
 
